Add FAA returns 4 example to demo.v

talks/demo/demo.v
@@ -1,9 +1,10 @@
-From iris.base_logic.lib Require Import invariants ghost_var.
+From iris.algebra.lib Require Import excl_auth.
+From iris.base_logic.lib Require Import invariants.
 From iris.heap_lang Require Import lib.par proofmode notation.
 Set Default Proof Using "All".
 Open Scope Z.
 
-(*! Part1: verifying swap *)
+(*! Part 1: verifying swap *)
 
 
 (** * The swap function, defined as a heap-lang value. *)
@@ -63,7 +64,7 @@ End proof.
 
 
 
-(*! Part2: verifying parallel add 2 example *)
+(*! Part 2: verifying parallel add 2 example *)
 
 Definition parallel_add : expr :=
   let: "r" := ref #0 in
@@ -80,6 +81,8 @@ Section proof.
     (∃ n : Z, r ↦ #n ∗ ⌜ Zeven n ⌝)%I.
 
   (** * main body of the proof *)
+  (* [inv N P] was written as a box around [P] (with no name [N]) in the
+  lecture *)
   Lemma faa_preserves_even (r : loc) :
     {{{ inv N (parallel_add_inv r) }}}
       FAA #r #2
@@ -87,8 +90,7 @@ Section proof.
   Proof.
     iIntros (Φ) "#Hinv Post".
     iInv "Hinv" as (n) ">[Hr %]".
-    wp_apply (wp_faa with "Hr").
-    iIntros "Hr".
+    wp_faa.
     iModIntro.
     iSplitL "Hr".
     { iNext. iExists (n + 2); iFrame.
@@ -96,7 +98,7 @@ Section proof.
     by iApply "Post".
   Qed.
 
-  Lemma parallel_add_spec :
+  Lemma parallel_add_spec_even :
     {{{ True }}} parallel_add {{{ n, RET #n; ⌜Zeven n⌝ }}}.
   Proof.
     iIntros (Φ) "_ Post".
@@ -120,6 +122,101 @@ Section proof.
     iModIntro.
     iSplitL "Hr".
     { iExists _; by iFrame. }
+    iApply "Post".
+    done.
+  Qed.
+End proof.
+
+
+
+(*! Part 3: verifying parallel add returns 4 *)
+Section proof.
+  Context `{!heapG Σ, !spawnG Σ, !inG Σ (excl_authR ZO)}.
+
+  Let N := nroot.@"example2".
+
+  (* [●E n] and [◯E n] are elements of the particular RA we used in
+  lecture to derive ghost variables, written ●n and ◯n in lecture *)
+  (* [own γ (●E n)] was written like γ ↪● n in the lecture *)
+
+  Definition parallel_add_inv_2 (r : loc) (γ1 γ2 : gname)
+    : iProp Σ :=
+    ∃ (n1 n2 : Z), r ↦ #(n1 + n2) ∗
+                   own γ1 (●E n1) ∗ own γ2 (●E n2).
+
+  (* these are the three lemmas for ghost variables, derived from the
+     general axioms for ownership *)
+
+  Lemma ghost_var_alloc (n : Z) :
+    True ==∗ ∃ γ, own γ (●E n) ∗ own γ (◯E n).
+  Proof.
+    iIntros "_".
+    iMod (own_alloc (●E n ⋅ ◯E n)) as (γ) "[H● H◯]".
+    { apply excl_auth_valid. }
+    iModIntro. iExists _; iFrame.
+  Qed.
+
+  Lemma ghost_var_agree (γ : gname) (n1 n2 : Z) :
+    own γ (●E n1) ∗ own γ (◯E n2) -∗ ⌜n1 = n2⌝.
+  Proof.
+    iIntros "[H1 H2]".
+    iDestruct (own_valid_2 with "H1 H2") as %H.
+    apply excl_auth_agree_L in H; done.
+  Qed.
+
+  Lemma ghost_var_update (n' : Z) (γ : gname) (n : Z) :
+    own γ (●E n) ∗ own γ (◯E n) ==∗ own γ (●E n') ∗ own γ (◯E n').
+  Proof.
+    iIntros "[H1 H2]".
+    iMod (own_update_2 _ _ _ (●E n' ⋅ ◯E n') with "H1 H2")
+      as "[H1 H2]".
+    { apply excl_auth_update. }
+    by iFrame.
+  Qed.
+
+  Lemma parallel_add_spec :
+    {{{ True }}} parallel_add {{{ n, RET #n; ⌜n = 4⌝ }}}.
+  Proof.
+    iIntros (Φ) "_ Post".
+    unfold parallel_add.
+    wp_alloc r as "Hr".
+    wp_let.
+    iMod (ghost_var_alloc 0 with "[//]") as (γ1) "[Hγ1● Hγ1◯]".
+    iMod (ghost_var_alloc 0 with "[//]") as (γ2) "[Hγ2● Hγ2◯]".
+    iMod (inv_alloc N _ (parallel_add_inv_2 r γ1 γ2) with "[Hr Hγ1● Hγ2●]") as "#Hinv".
+    { iNext. iExists _, _; iFrame. }
+    (* note that we have pre- and postconditions for each thread here,
+    reporting what each thread contributed *)
+    wp_apply (wp_par (λ _, own γ1 (◯E 2))%I (λ _, own γ2 (◯E 2))%I with
+                  "[Hγ1◯] [Hγ2◯]").
+
+    { iInv "Hinv" as (n1 n2) ">(Hr & Hγ1 & Hγ2)".
+      wp_faa.
+      iDestruct (ghost_var_agree with "[$Hγ1 $Hγ1◯]") as %->.
+      iMod (ghost_var_update 2 with "[$Hγ1 $Hγ1◯]") as "[Hγ1 Hγ1◯]".
+      iFrame "Hγ1◯".
+      iModIntro. iNext. iExists _, _; iFrame.
+      replace (2 + n2) with (0 + n2 + 2) by lia.
+      iAssumption. }
+
+    { iInv "Hinv" as (n1 n2) ">(Hr & Hγ1 & Hγ2)".
+      wp_faa.
+      iDestruct (ghost_var_agree with "[$Hγ2 $Hγ2◯]") as %->.
+      iMod (ghost_var_update 2 with "[$Hγ2 $Hγ2◯]") as "[Hγ2 Hγ2◯]".
+      iFrame "Hγ2◯".
+      iModIntro. iNext. iExists _, _; iFrame.
+      replace (n1 + 2) with (n1 + 0 + 2) by lia.
+      iAssumption. }
+
+    iIntros (v1 v2) "[Hγ1◯ Hγ2◯] !>".
+    wp_seq.
+    iInv "Hinv" as (n1 n2) ">(Hr & Hγ1 & Hγ2)".
+    iDestruct (ghost_var_agree with "[$Hγ1 $Hγ1◯]") as %->.
+    iDestruct (ghost_var_agree with "[$Hγ2 $Hγ2◯]") as %->.
+    wp_load.
+    iModIntro.
+    iSplitL "Hr Hγ1 Hγ2".
+    { iNext. iExists _, _; iFrame. }
     iApply "Post".
     done.
   Qed.
